

Hotelling's T^2 :

$$T_{cal}^2 = T^2 = n(\bar{X} - \mu_0)' S^{-1} (\bar{X} - \mu_0)$$

$$T_{tab}^2 = T_{n-1}^2 = \frac{(n-1)p}{n-p} F_{p, n-p; 0.05}$$

$$F_{p, n-p; 0.05} = F_{val} < -qf(p = 0.95, df1 = p, df2 = n - p)$$

Simultaneous confidence intervals:

95% confidence interval for μ_i :-

$$\bar{X}_i \mp \sqrt{T_{tab}^2 \frac{S_{ii}}{n}} \leq \mu_i$$

95% confidence interval for $\mu_i - \mu_j$:-

$$S_{pp} = S_{ii} * S_{jj} - 2S_{ij}$$

$$(\bar{X}_i - \bar{X}_j) \mp \sqrt{T_{tab}^2 \frac{S_{pp}}{n}} \leq \mu_i - \mu_j$$

Multivariate regression:

$$\hat{\beta} = (X'X)^{-1} X'Y$$

$$\hat{Y} = X\hat{\beta}$$

$$\hat{\epsilon} = Y - \hat{Y}$$

Total SS and cross-products = $Y'Y$

Predicted SS and cross-products = $\hat{Y}'\hat{Y}$

Residual SS and cross-products = $\hat{\epsilon}'\hat{\epsilon}$

$$Y'Y = \hat{Y}'\hat{Y} + \hat{\epsilon}'\hat{\epsilon}$$

MANOVA:

$$W = (n_1 - 1)S_1 + (n_2 - 1)S_2 + \cdots \cdots \cdots + (n_g - 1)S_g$$

$$\overline{X} = \frac{n_1\overline{X_1} + n_2\overline{X_2} + n_3\overline{X_3}}{n_1 + n_2 + n_3}$$

$$\boldsymbol{B} = \sum_{i=1}^g n_i(\overline{\boldsymbol{X}_i} - \overline{\boldsymbol{X}})(\overline{\boldsymbol{X}_i} - \overline{\boldsymbol{X}})'$$

$$\Lambda^* = \frac{|\boldsymbol{W}|}{|\boldsymbol{B} + \boldsymbol{W}|}$$

$$\text{The test statistics is} = \left(\frac{\sum n_i - p - 2}{p}\right) \left(\frac{1 - \sqrt{\Lambda^*}}{\sqrt{\Lambda^*}}\right)$$

$$F_{tab} = F_{2p,2(n-p-2;0.01)} = \frac{\chi^2_{2p;0.01}}{2p}$$

$$\text{Bartlett's (বারটলেটস) correction} = \chi^2_{cal} = -\left(n-1-\frac{p+g}{2}\right)\ln \Lambda^*$$

$$\chi^2_{tab} = \chi^2_{p(g-1);\alpha}$$

$$95\% \text{ simultaneous confidence interval for } \overline{X}_{kj} - \overline{X}_{li}$$

$$\overline{X}_{kj} - \overline{X}_{li} \pm t_{n-g}\left(\frac{\alpha}{pg(g-1)}\right)\sqrt{\frac{w_{jj}}{n-g}\left(\frac{1}{n_k} + \frac{1}{n_l}\right)}$$

$$\widehat{\boldsymbol{\tau}_{\boldsymbol{y}=x_j}} = [\overline{\boldsymbol{X}_l} - \overline{\boldsymbol{X}}]$$

$$\textbf{Box's test:}$$

$$S_{pooled} = \frac{(n_1-1)S_1 + (n_2-1)S_2 + (n_3-1)S_3}{n-g}$$

$$M = \left[\sum_l (n_l - 1) \right] \ln |S_{\text{pooled}}| - \sum_l [(n_l - 1) \ln |S_l|]$$

$$u=\left[\sum_l\frac{1}{n_l-1}-\frac{1}{\sum_l(n_l-1)}\right]\left[\frac{2p^2+3p-1}{6(p+1)(g-1)}\right]$$

$$\chi^2_{cal} = C = (1-u)M$$

$$\chi^2_{tab} = \chi^2_{\frac{p(p+1)(g-1)}{2};\alpha}$$